adapt to improved Imperative-HOL-Time

Refine_Imperative_HOL/IICF/Impl/IICF_Array_Matrix.thy
@@ -34,7 +34,7 @@ begin
   }"*)
 
 
-partial_function (heap) imp_for' :: "nat \<Rightarrow> nat \<Rightarrow> (nat \<Rightarrow> 'a \<Rightarrow> 'a Heap) \<Rightarrow> 'a \<Rightarrow> 'a Heap" where
+partial_function (heap_time) imp_for' :: "nat \<Rightarrow> nat \<Rightarrow> (nat \<Rightarrow> 'a \<Rightarrow> 'a Heap) \<Rightarrow> 'a \<Rightarrow> 'a Heap" where
   "imp_for' i u f s = (if i \<ge> u then return s else f i s \<bind> imp_for' (i + 1) u f)"
 
 declare imp_for'.simps[code]
